feat : added perm lemma for ndctx

src/rules/LJFC_Rules.v
@@ -30,8 +30,13 @@ Definition ndctx_insert (A : o) (C : ndctx) : ndctx :=
 Lemma ndctx_eq : forall (C1 C2 : ndctx),
     ndctx_list C1 = ndctx_list C2 -> C1 = C2.
 Proof.
-    intros [l1 p1] [l2 p2] H. simpl in H. subst.
-    f_equal. apply proof_irrelevance.
+    intros. simpl in H. 
+    destruct C1.
+    destruct C2.
+    simpl in H.
+    subst.
+    f_equal. 
+    apply proof_irrelevance.
 Qed.
 
 
@@ -146,3 +151,84 @@ with rfcC : ndctx -> o -> Prop :=
   forall {C: ndctx},
     rfcC C TT
 .
+
+Lemma ndctx_insert_perm_cons : 
+  forall (B : o) (C C' : ndctx),
+  Permutation C C' ->
+  Permutation (ndctx_insert B C) (ndctx_insert B C').
+Proof.
+  intros. simpl. unfold raw_insert. unfold ndctx_list in *.
+  destruct (in_dec o_eq_dec B (proj1_sig C)), (in_dec o_eq_dec B (proj1_sig C')).
+  - apply H.
+  - exfalso. apply n. eapply Permutation_in. apply H. apply i.
+  - exfalso. apply n. eapply Permutation_in. apply Permutation_sym. apply H. apply i.
+  - apply Permutation_cons. reflexivity. apply H.
+Qed.
+
+Lemma ndctx_insert_swap : forall (B1 B2 : o) (C : ndctx),
+  Permutation (ndctx_insert B1 (ndctx_insert B2 C)) (ndctx_insert B2 (ndctx_insert B1 C)).
+Proof.
+  intros. simpl. unfold raw_insert.
+  destruct 
+  (in_dec o_eq_dec B1),
+  (in_dec o_eq_dec B2 (proj1_sig C)).
+  - destruct
+    (in_dec o_eq_dec B2),
+    (in_dec o_eq_dec B1 (proj1_sig C)).
+    + apply Permutation_refl.
+    + contradiction.
+    + contradiction.
+    + contradiction.
+  - destruct
+    (in_dec o_eq_dec B2),
+    (in_dec o_eq_dec B1 (proj1_sig C)).
+    + contradiction.
+    + apply in_inv in i. destruct i.
+      -- subst. apply Permutation_cons. reflexivity. apply Permutation_refl.
+      -- contradiction.
+    + apply Permutation_cons. reflexivity. apply Permutation_refl.
+    + apply in_inv in i. destruct i.
+      -- subst. exfalso. apply n0. apply in_eq.
+      -- contradiction.
+  - destruct
+    (in_dec o_eq_dec B2),
+    (in_dec o_eq_dec B1 (proj1_sig C)).
+    + contradiction.
+    + apply Permutation_cons. reflexivity. apply Permutation_refl.
+    + contradiction.
+    + exfalso. apply n0. apply in_cons. apply i.
+  - destruct
+    (in_dec o_eq_dec B2),
+    (in_dec o_eq_dec B1 (proj1_sig C)).
+    + contradiction.
+    + apply in_inv in i. destruct i.
+      -- subst. exfalso. apply n. apply in_eq.
+      -- contradiction.
+    + exfalso. apply n. apply in_cons. apply i.
+    + apply perm_swap.
+Qed.
+
+Lemma ndctx_insert_perm_swap : 
+  forall (B1 B2 : o) (C C' : ndctx),
+  Permutation (ndctx_insert B2 (ndctx_insert B1 C)) C' ->
+  Permutation (ndctx_insert B1 (ndctx_insert B2 C)) C'.
+Proof.
+  intros.
+  transitivity (ndctx_insert B2 (ndctx_insert B1 C)).
+  - apply ndctx_insert_swap.
+  - apply H.
+Qed.
+
+Definition mk_ndctx (C : sctx) : ndctx :=
+    exist _ (nodup o_eq_dec C) (NoDup_nodup o_eq_dec C).
+
+Lemma ndctx_insert_mk_ndctx_eq : forall B C,
+    ndctx_insert B (mk_ndctx C) = mk_ndctx (B :: C).
+Proof.
+    intros. apply ndctx_eq. simpl. unfold raw_insert.
+    destruct (in_dec o_eq_dec B (nodup o_eq_dec C)).
+    - rewrite nodup_In in i.
+        destruct (in_dec o_eq_dec B C). reflexivity. contradiction.
+    - rewrite nodup_In in n.
+        destruct (in_dec o_eq_dec B C). contradiction. reflexivity.
+Qed.
