src/proofsearch/Sequents.v
@@ -1,0 +1,25 @@
+From Stdlib Require Import List.
+From LJF Require Import SharedLogic LJFC_Rules.
+
+Inductive sequent : Type :=
+| SbctC : forall {C L D}, bctC C L D -> sequent
+| SeptC : forall {C L D}, eptC C L D -> sequent
+| SlfcC : forall {C N K}, lfcC C N K -> sequent
+| SrfcC : forall {C P}, rfcC C P   -> sequent
+.
+
+Definition phase_rank (s : sequent) : nat :=
+    match s with
+    | SbctC _ => 1
+    | SeptC _ => 0
+    | SlfcC _ => 3
+    | SrfcC _ => 2
+    end
+.
+
+
+
+
+
+
+
